test/PolyTest.v
@@ -8,10 +8,12 @@ Require Import Tactics.
 From mathcomp Require Import all_ssreflect.
 Set Bullet Behavior "Strict Subproofs".
 
+Definition a : vty := vty_var "a"%string.
+
 (*Test 1: forall (x: 'a), x = x*)
 Module TestMonoId.
 
-Definition a : vty := vty_var "a"%string.
+
 Definition a' : vty := tyconst "'a".
 
 Definition x : vsymbol := ("x"%string, a).
@@ -39,3 +41,102 @@ Proof.
 Qed.
 
 End TestMonoId.
+
+(*Second test: very easy specialization of hypothesis*)
+Module TestSpecialize.
+
+Local Open Scope string_scope.
+
+(*Here, we assume that we have f : 'a -> int and g : 'a -> int
+  with the specification that forall x, f x = g x.
+  We prove that f 0 = g 0*)
+
+Definition f : funsym := funsym_noty "f" [a] vty_int.
+Definition g: funsym := funsym_noty "g" [a] vty_int.
+Definition x: vsymbol := ("x", a).
+Definition zero : term := Tconst (ConstInt 0).
+
+Definition spec_theory : theory :=
+  rev [tdef (abs_fun f); tdef (abs_fun g);
+  tprop Paxiom "fg_eq" 
+    (Fquant Tforall x (Feq vty_int (Tfun f [a] [Tvar x]) (Tfun g [a] [Tvar x])));
+    tprop Pgoal "fg_eq_int" (Feq vty_int (Tfun f [vty_int] [zero])
+      (Tfun g [vty_int] [zero]))].
+
+Lemma spec_theory_typed : typed_theory spec_theory.
+Proof.
+  check_theory.
+Qed.
+
+Lemma spec_theory_valid: valid_theory spec_theory.
+Proof.
+  simpl. split.
+  - wstart. wspecialize_ty "fg_eq" [("a", vty_int)].
+    unfold TySubst.ty_subst_wf_fmla. simpl_ty_subst.
+    simpl_ty_subst.
+    wspecialize "fg_eq" zero.
+    wassumption.
+  - split; auto. prove_axiom_wf.
+Qed.
+
+End TestSpecialize.
+
+(*Finally we combine them to show that we can prove
+  polymorphic goals with polymorphic assumptions.
+  We prove that any function that is involutive is injective*)
+
+Module InjTest.
+Local Open Scope string_scope.
+
+Definition f : funsym := funsym_noty "f" [a] a.
+Definition x: vsymbol := ("x", a).
+Definition y: vsymbol := ("y", a).
+
+Definition inj_theory : theory :=
+  rev [
+    tdef (abs_fun f);
+    tprop Paxiom "f_inv" (Fquant Tforall x (Feq a 
+      (Tfun f [a] [Tfun f [a] [Tvar x]])
+      (Tvar x)));
+    tprop Plemma "f_inj" (fforalls [x; y]
+      (Fbinop Timplies 
+        (Feq a (Tfun f [a] [Tvar x]) (Tfun f [a] [Tvar y]))
+        (Feq a (Tvar x) (Tvar y))))
+  ].
+
+Lemma inj_theory_typed : typed_theory inj_theory.
+Proof.
+  check_theory.
+Qed.
+
+Definition a' := tyconst "a".
+Definition x' := ("x", a').
+Definition y' := ("y", a').
+Definition x'' := constsym "x" a'.
+Definition y'' := constsym "y" a'.
+Definition x1 := Tfun x'' nil nil.
+Definition y1 := Tfun y'' nil nil.
+Ltac extra_simpl ::= fold a'; fold x'; fold y'; fold x''; 
+unfold t_constsym ; fold y''; fold x1; fold y1.
+
+Lemma inj_theory_valid: valid_theory inj_theory.
+Proof.
+  simpl. split; [| split; auto; prove_axiom_wf].
+  exists ["a"].
+  wstart.
+  (*First, specialize f_inv to a*)
+  wspecialize_ty "f_inv" [("a", tyconst "a")].
+  (*? Why didn't this run*)
+  simpl_ty_subst.
+  wcopy "f_inv" "f_inv2". simpl. (*TODO: add to copy*)
+  wintros "x" "y".
+  wintros "Heq".
+  wspecialize "f_inv" x1.
+  wrewrite<- "f_inv".
+  wrewrite "Heq".
+  wspecialize "f_inv2" y1.
+  wrewrite "f_inv2".
+  wreflexivity.
+Qed.
+
+End InjTest.
